src/BasicProg.v
@@ -8,6 +8,7 @@ Require Import Nomega.
 Require Import NArith.
 Require Import FunctionalExtensionality.
 Require Import List.
+Require Import EqdepFacts.
 
 Set Implicit Arguments.
 
@@ -146,6 +147,30 @@ Proof.
 Qed.
 
 Hint Extern 1 ({{_}} progseq (Trim _) _) => apply trim_ok : prog.
+
+Theorem hash_ok:
+  forall sz (buf : word sz),
+  {< (_ : unit),
+  PRE         emp
+  POST RET:r  emp * [[ hash_inv r = existT _ sz buf ]] * [[ hash_fwd buf = r ]]
+  CRASH       emp
+  >} Hash buf.
+Proof.
+  unfold corr2; intros.
+  destruct_lift H.
+  inv_exec.
+  - inv_step.
+    eapply H4; eauto.
+    pred_apply. cancel.
+    pose proof (eq_sigT_snd H5).
+    autorewrite with core in *. congruence.
+  - exfalso.
+    apply H5. repeat eexists.
+  - right. eexists; intuition eauto.
+    pred_apply. cancel.
+Qed.
+
+Hint Extern 1 ({{_}} progseq (Hash _) _) => apply hash_ok : prog.
 
 Definition If_ {PROGTYPE : Type -> Type} {T : Type} P Q (b : {P} + {Q}) (p1 p2 : PROGTYPE T) :=
   if b then p1 else p2.
